ulib/experimental/Steel.SelEffect.fsti
@@ -252,12 +252,12 @@ unfold
 let vptr r = VUnit (vptr' r)
 
 val alloc (#a:Type0) (x:a) : SteelSel (ref a)
-  vemp (fun r -> vptr r)
+  emp (fun r -> vptr r)
   (requires fun _ -> True)
   (ensures fun _ r h1 -> h1 (vptr r) == x /\ not (R.is_null r))
 
 val free (#a:Type0) (r:ref a) : SteelSel unit
-  (vptr r) (fun _ -> vemp)
+  (vptr r) (fun _ -> emp)
   (requires fun _ -> True)
   (ensures fun _ _ _ -> True)
 
